Verified parser combinators

opentheory/examples/all.ml
@@ -4,10 +4,10 @@
 
 start_logging ();;
 
+loads "opentheory/examples/parser.ml";;
 loads "opentheory/examples/modular.ml";;
 loads "opentheory/examples/word.ml";;
 loads "opentheory/examples/byte.ml";;
-loads "opentheory/examples/parser.ml";;
 loads "opentheory/examples/char.ml";;
 
 stop_logging ();;
